plf/Makefile.coq
@@ -44,7 +44,7 @@ HASNATDYNLINK     := $(COQMF_HASNATDYNLINK)
 OCAMLWARN         := $(COQMF_WARN)
 
 Makefile.coq.conf: 
-	/snap/coq-prover/15/coq-platform/2021-02-1/bin/coq_makefile COQBIN = /snap/coq-prover/15/coq-platform/2021-02-1/bin/ -Q . PLF -o Makefile.coq Maps.v Imp.v Preface.v Equiv.v Hoare.v Hoare2.v HoareAsLogic.v Smallstep.v Types.v Stlc.v StlcProp.v MoreStlc.v Sub.v Typechecking.v Records.v References.v RecordSub.v Norm.v PE.v Postscript.v Bib.v LibTactics.v UseTactics.v UseAuto.v MapsTest.v ImpTest.v PrefaceTest.v EquivTest.v HoareTest.v Hoare2Test.v HoareAsLogicTest.v SmallstepTest.v TypesTest.v StlcTest.v StlcPropTest.v MoreStlcTest.v SubTest.v TypecheckingTest.v RecordsTest.v ReferencesTest.v RecordSubTest.v NormTest.v PETest.v PostscriptTest.v BibTest.v LibTacticsTest.v UseTacticsTest.v UseAutoTest.v
+	/snap/coq-prover/27/coq-platform/2021-09-0/bin/coq_makefile COQBIN = /snap/coq-prover/27/coq-platform/2021-09-0/bin/ -Q . PLF -o Makefile.coq Maps.v Imp.v Preface.v Equiv.v Hoare.v Hoare2.v HoareAsLogic.v Smallstep.v Types.v Stlc.v StlcProp.v MoreStlc.v Sub.v Typechecking.v Records.v References.v RecordSub.v Norm.v PE.v Postscript.v Bib.v LibTactics.v UseTactics.v UseAuto.v MapsTest.v ImpTest.v PrefaceTest.v EquivTest.v HoareTest.v Hoare2Test.v HoareAsLogicTest.v SmallstepTest.v TypesTest.v StlcTest.v StlcPropTest.v MoreStlcTest.v SubTest.v TypecheckingTest.v RecordsTest.v ReferencesTest.v RecordSubTest.v NormTest.v PETest.v PostscriptTest.v BibTest.v LibTacticsTest.v UseTacticsTest.v UseAutoTest.v
 
 # This file can be created by the user to hook into double colon rules or
 # add any other Makefile code he may need
